More direct model of machine integers

src/Helpers/MachinePrimitives.v
@@ -2,59 +2,144 @@
 Global Unset Auto Template Polymorphism.
 Global Set Implicit Arguments.
 
+From Coq Require Import Omega.
+From Coq Require Import Nat.
 From Classes Require Import EqualDec.
-
 From stdpp Require Import decidable countable.
 
 Instance eqdecision `{dec:EqualDec A} : EqDecision A := dec.
 
-From Coq Require Import NArith.NArith.
-Local Open Scope N.
-
 (** Machine unsigned integers *)
 
-Record MachineUInt (bytes:nat) : Type :=
-  { intTy :> Type;
-    intPlus : intTy -> intTy -> intTy;
-    intSub : intTy -> intTy -> intTy;
-    intCmp : intTy -> intTy -> comparison;
-    fromNum : N -> intTy;
-    int_val0 := fromNum 0;
-    int_val1 := fromNum 1;
-    toNum : intTy -> N;
-    toNum_inj : forall x y, toNum x = toNum y -> x = y;
-    intCmp_ok : forall x y, intCmp x y = N.compare (toNum x) (toNum y);
-    toNum_ok : forall x, toNum x < N.pow 2 (8 * N.of_nat bytes);
-  }.
+Module UInt.
+  Definition max bytes_m1 := pow 2 (8 + 8 * bytes_m1).
+  Record t (bytes_m1:nat) :=
+    mk { val : nat;
+         val_wf : val < max bytes_m1; }.
+End UInt.
 
-Arguments int_val0 {bytes int} : rename.
-Arguments int_val1 {bytes int} : rename.
-Arguments intCmp {bytes int} : rename.
-Arguments intSub {bytes int} : rename.
-Arguments toNum {bytes int} : rename.
+Arguments UInt.mk bytes_m1 val val_wf : clear implicits.
 
-Instance uint_eqdec bytes (int: MachineUInt bytes) : EqualDec int.
+Definition uint := UInt.t.
+
+Section uint.
+  Context {bytes_m1:nat}.
+  Notation t := (uint bytes_m1).
+  Notation mk := (UInt.mk bytes_m1).
+  Notation val := (@UInt.val bytes_m1).
+  Notation bound := (UInt.max bytes_m1).
+
+  Implicit Types (x y:t).
+
+  Lemma bound_not_0 : bound <> 0.
+  Proof.
+    unfold bound.
+    apply Nat.pow_nonzero.
+    auto.
+  Qed.
+
+  Lemma bound_gt_1 : 1 < bound.
+  Proof.
+    unfold bound.
+    change (8 + 8 * bytes_m1) with (1 + (7 + 8 * bytes_m1)).
+    rewrite Nat.pow_add_r.
+    generalize dependent (7 + 8 * bytes_m1); intros.
+    assert (2 ^ n <> 0).
+    apply Nat.pow_nonzero; auto.
+    generalize dependent (2 ^ n); intros.
+    simpl.
+    lia.
+  Qed.
+
+  Lemma bound_gt_0 : 0 < bound.
+    pose proof bound_gt_1.
+    lia.
+  Qed.
+
+  Hint Resolve bound_not_0 bound_gt_0 : core.
+
+  Tactic Notation "mkT" uconstr(x) := refine (mk x _).
+
+  Definition intPlus x y : t.
+    mkT ((x.(val) + y.(val)) mod bound).
+    apply Nat.mod_upper_bound; auto.
+  Defined.
+
+  Definition intSub x y : t.
+    mkT (x.(val) - y.(val)).
+    pose proof UInt.val_wf x.
+    abstract lia.
+  Defined.
+
+  Definition fromNum (n:nat) : t.
+    mkT (n mod bound).
+    apply Nat.mod_upper_bound; auto.
+  Defined.
+
+  Definition int_val0 : t.
+    mkT 0.
+    auto.
+  Defined.
+
+  Definition int_val1 : t.
+    mkT 1.
+    apply bound_gt_1.
+  Defined.
+
+  Definition intCmp x y : comparison :=
+    Nat.compare x.(val) y.(val).
+
+  Definition toNum x : nat := x.(val).
+
+  Theorem toNum_inj : forall x y, toNum x = toNum y -> x = y.
+  Proof.
+    intros.
+    destruct x as [x Hx], y as [y Hy]; simpl in *.
+    subst; auto.
+    f_equal.
+    apply proof_irrel.
+  Qed.
+
+  Global Instance uint_eq_dec : EqualDec t.
+  apply (EqualDec.inj_eq_dec toNum toNum_inj).
+  Defined.
+
+End uint.
+
+Definition uint64 := UInt.t (8 - 1).
+Definition uint32 := UInt.t (4 - 1).
+Definition uint16 := UInt.t (2 - 1).
+Definition uint8  := UInt.t (1 - 1).
+
+Definition uint_val4096 : uint64 := fromNum 4096.
+
+Definition uint64_to_uint16 (x:uint64) : uint16 :=
+  fromNum x.(UInt.val).
+
+Definition uint64_to_uint32 (x:uint64) : uint32 :=
+  fromNum x.(UInt.val).
+
+Definition upcast_bound {bytes_m1_1 bytes_m1_2} :
+  forall x, x < UInt.max bytes_m1_1 ->
+       bytes_m1_1 <= bytes_m1_2 ->
+       x < UInt.max bytes_m1_2.
 Proof.
-  hnf; intros.
-  destruct_with_eqn (intCmp x y);
-    [ left | right; intros -> .. ];
-    rewrite intCmp_ok, ?N.compare_eq_iff, ?N.compare_refl in *.
-  - auto using toNum_inj.
-  - congruence.
-  - congruence.
+  intros.
+  unfold UInt.max in *.
+  eapply Nat.lt_le_trans; eauto.
+  apply Nat.pow_le_mono_r; auto.
+  lia.
+Qed.
+
+Definition uint16_to_uint64 (x:uint16) : uint64.
+  refine (UInt.mk _ x.(UInt.val) _).
+  apply (upcast_bound x.(UInt.val_wf)); abstract (simpl; repeat constructor).
 Defined.
 
-Axiom uint64 : MachineUInt 8.
-Axiom uint32 : MachineUInt 4.
-Axiom uint16 : MachineUInt 2.
-Axiom uint8  : MachineUInt 1.
-
-Definition uint_val4096 : uint64 := uint64.(fromNum) 4096.
-
-Axiom uint64_to_uint16 : uint64 -> uint16.
-Axiom uint64_to_uint32 : uint64 -> uint32.
-Axiom uint16_to_uint64 : uint16 -> uint64.
-Axiom uint32_to_uint64 : uint32 -> uint64.
+Definition uint32_to_uint64 (x:uint32) : uint64.
+  refine (UInt.mk _ x.(UInt.val) _).
+  apply (upcast_bound x.(UInt.val_wf)); abstract (simpl; repeat constructor).
+Defined.
 
 Axiom ByteString : Type.
 Axiom eqdec_ByteString : EqualDec ByteString.
@@ -77,17 +162,17 @@ Module BSNotations.
   Infix "++" := BS.append : bs_scope.
 End BSNotations.
 
-Class UIntEncoding bytes (int: MachineUInt bytes) : Type :=
-  { encodeLE : int -> ByteString;
-    decodeLE : ByteString -> option int;
-    encode_length_ok : forall x, toNum (BS.length (encodeLE x)) = N.of_nat bytes;
+Class UIntEncoding bytes_m1 : Type :=
+  { encodeLE : UInt.t bytes_m1 -> ByteString;
+    decodeLE : ByteString -> option (UInt.t bytes_m1);
+    encode_length_ok : forall x, toNum (BS.length (encodeLE x)) = 1 + bytes_m1;
     encode_decode_LE_ok : forall x, decodeLE (encodeLE x) = Some x;
   }.
 
-Axiom uint64_le_enc : UIntEncoding uint64.
-Axiom uint32_le_enc : UIntEncoding uint32.
-Axiom uint16_le_enc : UIntEncoding uint16.
-Axiom uint8_le_enc : UIntEncoding uint8.
+Axiom uint64_le_enc : UIntEncoding (8 - 1).
+Axiom uint32_le_enc : UIntEncoding (4 - 1).
+Axiom uint16_le_enc : UIntEncoding (2 - 1).
+Axiom uint8_le_enc : UIntEncoding (1 - 1).
 Existing Instances uint64_le_enc uint32_le_enc uint16_le_enc uint8_le_enc.
 
 (** File descriptors *)
